\begin{proposition}
  For all \rchreqarng,
  $$\prop.$$%
\end{proposition}

\begin{proof}
  From the definition of conditional probability, we have
  $$ 
  \PSTT(\AV_\TT = \STT_\TT(\SS) \mid \SV_\TT = \SS)
  = 
  \frac
  {\PSTT(\AV_\TT = \STT_\TT(\SS), \SV_\TT = \SS)}
  {\PSTT(\SV_\TT = \SS)}.$$

  In one direction, we have that if $\PSTT(\SV_\TT = \SS) > 0$, then 
  $ \PSTT(\AV_\TT = \STT_\TT(\SS) \mid \SV_\TT = \SS) $
  is also defined because the denominator in the equation above is nonzero.

  In the other direction, we have that if $\PSTT(\SV_\TT = \SS) = 0$, then 
  $ \PSTT(\AV_\TT = \STT_\TT(\SS) \mid \SV_\TT = \SS) $
  is undefined because the denominator in the equation above is zero.

  Therefore, we have that
  $$\prop.$$%
\end{proof}
