\begin{proposition}
  \nrp 1
  We have that, \sqpevctoevexprprop.%
\end{proposition}

\begin{proof}
  \nrp 2
  We have that
  \begin{align*}
    \ESQ{\SQPP}{f} \relrg = {\mreflng{\probpath/proof/sqevexpr}} 12pt &
    \sum_{\pin\XX\X}\sum_{\pin\YY\Y}f(\XV = \XX,\YV = \YY)\times \MPRSQ{\SQPP}{\XV = \XX,\YV = \YY}\\
    \relrg = {\mrefmargzimpl} 12pt &
    \sum_{\pin\XX\X}\ \sum_{\pin\YY\Y : \MPRSQ{\SQPP}{\YV = \YY} > 0}f(\XV = \XX,\YV = \YY)\times \MPRSQ{\SQPP}{\XV = \XX,\YV = \YY}\\
    \relrg = {\mrefcprtompr} 12pt &
        \sum_{\pin\XX\X}\ \sum_{\pin\YY\Y : \MPRSQ{\SQPP}{\YV = \YY} > 0}f(\XV = \XX,\YV = \YY)\times \MPRSQ{\SQPP}{\YV = \YY}\times \CPRSQ{\SQPP}{\XV = \XX}{\YV = \YY}\\
      = &
        \sum_{\pin\YY\Y : \MPRSQ{\SQPP}{\YV = \YY} > 0}\MPRSQ{\SQPP}{\YV = \YY}\times \sum_{\pin\XX\X}\CPRSQ{\SQPP}{\XV = \XX}{\YV = \YY}f(\XV = \XX,\YV = \YY)\\
      \relrg = {\mreflng{\probpath/proof/sqevcexpr}} 12pt &
      \sum_{\pin\YY\Y : \MPRSQ{\SQPP}{\YV = \YY} > 0}\MPRSQ{\SQPP}{\YV = \YY} \times \ESQC{\SQPP}{f}{\YV = \YY}.
  \end{align*}
\end{proof}
