\begin{proposition}
  \nrp 1
  We have that, \indproddefa.%
\end{proposition}

\begin{proof}
  \hrule
  \nrp 2
  $\implies$ suppose $\rell {\CIND{\XV}{\YV}{\ZV}} f $.

  Then, for all $\xyzchoice$, there are two cases to consider:
  \begin{itemize}
    \item \nrp 4 $\CPr{\XV = \XX, \YV = \YY}{\ZV = \ZZ} \rell = fco \undef$.

      Then, 
      $\MPr{\ZZ} \rellr = zz {\mrefconddef} 0$,
      so
      $\CPr{\XX}{\ZZ} \relr = {\mrefconddef} \undef$
      and
      $\CPr{\YY}{\ZZ} \relr = {(zz)->\mrefconddef} \undef$, so
      \begin{align*}
        \CPr{\XX, \YY}{\ZZ}  \relr = fco \undef =
        \CPr{\XX}{\ZZ} \times \CPr{\YY}{\ZZ}.
      \end{align*}
    \item \nrp 5 $\CPr{\XV = \XX, \YV = \YY}{\ZV = \ZZ} \rell {\ne} fct \undef$.

      Then, we have $\MPr{\ZZ} \rellr > zg {\mrefconddef} 0$, so $\CPr{\YY}{\ZZ} \relr {\ne} {\mrefconddef} \undef$, and there are two cases to consider:
      \begin{itemize}
        \item \nrp 6 $\CPr{\YY}{\ZZ} \rell > fcto 0$.

        \nrp 7
        Then,
        \begin{align*}
          \MPr{\YY, \ZZ} \relr = {(zg)->\mrefcprtompr}
          \CPr{\YY}{\ZZ} \times \MPr{\ZZ} \rellr > yzg {fcto,zg} 0,
        \end{align*}
        \nrp 8
        so
        \begin{align*}
          \CPr{\XX, \YY}{\ZZ} 
          \relr = {(fcto)->\mrefccprtompr} &\ \CPr{\XX}{\YY, \ZZ} \times \CPr{\YY}{\ZZ}\\
          \relr = {((-yzg)->\mrefconddef)->f} &\ \CPr{\XX}{\ZZ} \times \CPr{\YY}{\ZZ}.
        \end{align*}

        \item \nrp 9 $\CPr{\YY}{\ZZ} \rell = {fctt} 0$.

        Then,
        \begin{align*}
          \CPr{\XX, \YY}{\ZZ} \relr = {\mrefcmarggimpl} \ \ \ \ \ 0\ \ \ \ \  
          \relr = {fctt,(zg)->\mrefconddef} \CPr{\XX}{\ZZ} \times \CPr{\YY}{\ZZ}.
        \end{align*}
      \end{itemize}
  \end{itemize}

  \hrule
  \nrp 10
  $\impliedby$ suppose 
  $$\forall \xyzchoice,
  \CPr{\XV = \XX, \YV = \YY}{\ZV = \ZZ} \rell = b 
  \CPr{\XV = \XX}{\ZV = \ZZ}
  \times
  \CPr{\YV = \YY}{\ZV = \ZZ}.$$

  Then, for all $\xyzchoice$, supposing $\CPr{\XV = \XX}{\YV = \YY, \ZV = \ZZ} \rell {\ne} ba \undef$, there are two cases to consider:
  \begin{itemize}
    \item \nrp 11 $\MPr{\ZZ} \rell > bco 0$.

      \nrp 12
      Then, we have that
      $$\CPr{\YY}{\ZZ} \relrg = {\mrefcondprob} 15pt \frac{\MPr{ \YY, \ZZ}}{\MPr{\ZZ}} \rellrg > ygzg -10pt {bco,(ba)->\mrefconddef} 15pt 0.$$
      \nrp 13
      so
      \begin{align*}
        \CPr{\XX}{\YY, \ZZ}
        \relrg = {\mrefccondprob} 15pt \ & 
        \frac{\CPr{\XX, \YY}{\ZZ}}{\CPr{\YY}{\ZZ}}
        \\
        \relr = b \ & \frac{\CPr{\XX}{\ZZ} \times \CPr{\YY}{\ZZ}}{\CPr{\YY}{\ZZ}}\\
        \relr = -ygzg \ & \CPr{\XX}{\ZZ}.
      \end{align*}
    \item \nrp 14 $\MPr{\ZZ} \rell = bct 0$.

      Then,
      \begin{align*}
        \CPr{\XX}{\YY, \ZZ}
        \relr = {((bct)->\mrefmargzimpl)->\mrefconddef}
        \ \ \ \ 
        \ \ 
        \undef
        \ \ \ \ 
        \ \ 
        \relr = {(bct)->\mrefconddef} \CPr{\XX}{\ZZ}.
      \end{align*}
  \end{itemize}
  \hrule
\end{proof}
\begin{proposition}
  \nrp 20
  We have that, \indproddefb.%
\end{proposition}
\begin{proof}
  \hrule
  \nrp 15
  $\implies$ suppose $\rell {\IND{\XV}{\YV}} f $.

  Then, for all $\xychoice$, there are two cases to consider:
  \begin{itemize}
    \item \nrp 16 $\MPr{\YY} \rell > fco 0$.

    Then,
    \begin{align*}
      \MPr{\XX, \YY}
      \relr = {\mrefcprtompr} &\ \CPr{\XX}{\YY} \times \MPr{\YY}\\
      \relr = {((fco)->\mrefconddef)->f} &\ \MPr{\XX} \times \MPr{\YY}.
    \end{align*}

    \item \nrp 17 $\MPr{\YY} \rell = fct 0$.

    Then,
    \begin{align*}
      \MPr{\XX, \YY} \relr = {\mrefmarggimpl} \ \ 0\ \ 
      \relr = fct \MPr{\XX} \times \MPr{\YY}.
    \end{align*}
  \end{itemize}

  \hrule
  \nrp 18
  $\impliedby$ suppose 
  $$\forall \xychoice,
  \MPr{\XV = \XX, \YV = \YY} \rell = b
  \MPr{\XV = \XX}
  \times
  \MPr{\YV = \YY}.$$

  \nrp 19
  Then, for all $\xychoice$, supposing $\CPr{\XV = \XX}{\YV = \YY} {\ne} \undef$, we have that
  $\MPr{\YY} \rellr > yg {\mrefconddef} 0,$
  so
  \begin{align*}
    \CPr{\XX}{\YY}
    \relrg = {\mrefcondprob} 15pt \ & 
    \frac{\MPr{\XX, \YY}}{\MPr{\YY}}
    \\
    \relr = b \ & \frac{\MPr{\XX} \times \MPr{\YY}}{\MPr{\YY}}\\
    \relr = yg \ & \MPr{\XX}.
  \end{align*}
  \hrule
\end{proof}
