\begin{proposition}
  \nrp 1
  We have that \pathuniqprop.%
\end{proposition}

\begin{proof}
  \hrule
  {\it Base case.}

  We have that, for all $\PTH \in \ALLPATHS$ such that $\OSS{\PTH} \rell = bc 1 $,
  letting 
  $\PTHP \rell {\defeq} pe \PTH$,
  we have 
  $$\OSI{\PTHP}{0} \relr = pe \OSI{\PTH}{0},\OSI{\PTHP}{-1} \relr = pe \OSI{\PTH}{-1},$$
  so
  $$\relr {\PATHSEQ{\PTH}{\PTHP}} {\mrefpathseq} ,$$
  and, for all $\VTXX \in \PTH$
  $$1 \le \OSCNT{\VTXX}{\PTH} = \OSCNT{\VTXX}{\PTHP} \le \OSS{\PTHP} \relr = pe \OSS{\PTH} \relr = bc 1,$$%
  so
  $$\OSCNT{\VTXX}{\PTHP} = 1.$$
  \hrule
  {\it Inductive hypothesis.}

  Suppose, for all $1 \le \IHN' \le \IHN$, with $\IHN \ge 1$, and 
  all $\PTH \in \ALLPATHS$ such that $\OSS{\PTH} = \IHNP$,
  there exists $\PTHP \in \ALLPATHS$ such that
  $$\rell {\PATHSEQ{\PTH}{\PTHP}} iha \and \forall \VTXX \in \PTH, \OSCNT{\VTXX}{\PTHP} \rell = ihb 1 .$$
  \hrule
  {\it Inductive step.}

  We have that, for all $\PTH \in \ALLPATHS$ such that $\OSS{\PTH} = \IHN + 1$,
  there are two cases to consider:
  \begin{itemize}
    \item $\forall \VTXX \in \PTH, \OSCNT{\VTXX}{\PTH} = 1 .$

    Then, letting 
    $\PTHP \rell {\defeq} pe \PTH$,
    we immediately have
    $$\relr {\PATHSEQ{\PTH}{\PTHP}} {\mrefpathseq} \and \forall \VTXX \in \PTH, \OSCNT{\VTXX}{\PTHP} = \OSCNT{\VTXX}{\PTH} = 1.$$

    \item $\exists \VTXX \in \PTH : \OSCNT{\VTXX}{\PTH} > 1 .$

    Then, there are two cases to consider:
    \begin{itemize}
      \item $\VTXX = \OSI{\PTH}{0}$.
        Then, letting $\OSTT = \OSIGI{\PTH}{\VTXX}{1}$, we have that
        $$\OSI{\PTH}{\OSTT:} \relr {\in} {\mreflng{\grpath/proof/subpath}} \ALLPATHS,$$
        and letting
      \item $\VTXX \rell {\ne} fn \OSI{\PTH}{0}$.
        Then, letting $\OSTT_1 \rell {\defeq} to \OSIGI{\PTH}{\VTXX}{0}$
        and $\OSTT_2 \rell {\defeq} tt \OSIGI{\PTH}{\VTXX}{1}$,
        we have that
        $$\OS{\OSI{\PTH}{\OSTT_1 - 1}, \OSI{\PTH}{\OSTT_2}} = \OS{\OSI{\PTH}{\OSTT_1 - 1}, \OSI{\PTH}{\OSTT_1}} \rell {\in} ie \EDG,$$
        so
        $$\OSI{\PTH}{:\OSTT_1} \cup \OSI{\PTH}{\OSTT_2:} \relr {\in} {(\mreflng{\grpath/proof/subpath},ie)->\mreflng{\grpath/proof/subpathcomb}} \ALLPATHS,$$
        and letting
        $$\PTH^- \rell {\defeq} pm \OSI{\PTH}{:\OSTT_1} \cup \OSI{\PTH}{\OSTT_2:},$$
        we have
        $$\OSI{\PTH^-}{0} \relr = fn,to,pm \OSI{\PTH}{0} \and \OSI{\PTH^-}{-1} \relr = tt,pm \OSI{\PTH}{-1}
        \implies \PATHSEQ{\PTH}{\PTH^-}
        ,$$
        with
        $$\OSS{\PTH^-} < $$
    \end{itemize}
  \end{itemize}

  \hrule
\end{proof}
