\begin{proposition}
  We have that\ \cprsqexprprop.%
\end{proposition}

\begin{proof}
  \begin{align*}
    \CPRSQ{\SQPP}{f}{\YV = \YY} 
    \relrg = {\mreflng{definition}{\probpath/definition/cprsq}} 10pt \ & 
    \lim_{\TR \rightarrow \infty}
    \left(
    \frac
    {\sum_{\TR' = 1}^{\TR}\SQI{\SQPP}{\TR'}{\XV = \XX, \YV = \YY}}
    {\sum_{\TR' = 1}^{\TR}\SQIM{\SQPP}{\TR'}{\YV = \YY}}
    \right)\\
    = \ &
    \lim_{\TR \rightarrow \infty}
    \left(
    \frac
    {\left({\sum_{\TR' = 1}^{\TR}\SQI{\SQPP}{\TR'}{\XV = \XX, \YV = \YY}}\right)/{\TR}}
    {\left(\sum_{\TR' = 1}^{\TR}\SQIM{\SQPP}{\TR'}{\YV = \YY}\right)/\TR}
    \right)\\
    \relrg = {\mreflng{proof}{\probpath/proof/problimdef},\mreflng{proof}{\probpath/proof/mproblimdef}} 19pt \ & 
    \frac
    {
      \lim_{\TR \rightarrow \infty}\left(
    \left({\sum_{\TR' = 1}^{\TR}\SQI{\SQPP}{\TR'}{\XV = \XX, \YV = \YY}}\right)/{\TR}\right)}
    {
      \lim_{\TR \rightarrow \infty}\left(
    \left(\sum_{\TR' = 1}^{\TR}\SQIM{\SQPP}{\TR'}{\YV = \YY}\right)/\TR\right)}
    \\
    \relrg = {\mreflng{definition}{\probpath/definition/prsq},\mreflng{definition}{\probpath/definition/mprsq}} 15pt \ & 
    \frac { \PRSQ{\SQPP}{\XV = \XX, \YV = \YY} } { \MPRSQ{\SQPP}{\YV = \YY} }\\
  \end{align*}
\end{proof}
